fix: port the proofs to the map-reduce checker

Veil/Core/Tools/ModelChecker/ConcreteNew/MapReduce.lean
@@ -6,12 +6,6 @@ namespace Veil.ModelChecker.Concrete
 open Veil
 
 variable {ρ σ κ σₕ : Type} [fp : StateFingerprint σ σₕ] [BEq κ] [Hashable κ] [Ord σₕ]
-  (params : SearchParameters ρ σ) (th : ρ)
-
-@[inline]
-def MapReduceSearchContextMain.hasFinished (mctx : MapReduceSearchContextMain σ κ σₕ) : Bool :=
-  -- mctx.base.hasFinished
-  mctx.1.hasFinished
 
 @[inline]
 def MapReduceSearchContextLocal.hasFinished (lctx : MapReduceSearchContextLocal σ κ σₕ) : Bool :=
@@ -24,7 +18,6 @@ variable (globalSeen : Std.TreeSet σₕ)
 -- FIXME: The logic of `tryExploreNeighbor`, `processSuccessors`, and `processState`
 -- seems very similar to the sequential processing logic. We should try to unify them
 
-omit params th in
 /-- Process a single neighbor in the local context.
     `globalSeen` is the main context's log, used to check if a state is already globally seen. -/
 @[inline]
@@ -42,7 +35,6 @@ def MapReduceSearchContextLocal.tryExploreNeighbor
       actionStatsMap := ctx.actionStatsMap.update true label
     }, q.push ⟨fingerprint, succ, nextDepth⟩)
 
-omit params th in
 /-- Process all successors of a state in the local context. -/
 def MapReduceSearchContextLocal.processSuccessors
   (fpSt : σₕ) (depth : Nat)
@@ -55,6 +47,7 @@ def MapReduceSearchContextLocal.processSuccessors
 /-- Process a single state: check violations via BaseSearchContext.processState,
     then process successors if no early termination. -/
 def MapReduceSearchContextLocal.processState
+  (params : SearchParameters ρ σ) (th : ρ)
   (fpSt : σₕ) (depth : Nat) (curr : σ)
   (outcomes : List (κ × ExecutionOutcome ℤ σ))
   (lctx : MapReduceSearchContextLocal σ κ σₕ) : MapReduceSearchContextLocal σ κ σₕ :=
@@ -67,103 +60,512 @@ def MapReduceSearchContextLocal.processState
     let ctx'' := { ctx' with statesFound := ctx'.statesFound + successfulTransitions.length }
     MapReduceSearchContextLocal.processSuccessors globalSeen fpSt depth successfulTransitions (ctx'', q)
 
-def MapReduceSearchContextLocal.processWorkQueue
-  (outcomesComputer : ρ → σ → List (κ × ExecutionOutcome ℤ σ))
-  (queue : Array (QueueItem σₕ σ))
-  (lctx : MapReduceSearchContextLocal σ κ σₕ) : MapReduceSearchContextLocal σ κ σₕ := Id.run do
-  let mut res := lctx
-  for item in queue do
-    if res.hasFinished then break else pure ()
-    let ⟨fpSt, curr, depth⟩ := item
-    res := MapReduceSearchContextLocal.processState params th globalSeen fpSt depth curr (outcomesComputer th curr) res
-  return res
+end
 
-/-- Main worker entry point. Creates a neutral context and processes the work queue.
-    This function is called by each parallel task. -/
-def MapReduceSearchContextLocal.bfsBigStep
-  (outcomesComputer : ρ → σ → List (κ × ExecutionOutcome ℤ σ))
-  (completedDepth : Nat)
-  (queue : Array (QueueItem σₕ σ)) : MapReduceSearchContextLocal σ κ σₕ :=
-  let lctx : MapReduceSearchContextLocal σ κ σₕ := MapReduceSearchContextLocal.initial completedDepth
-  MapReduceSearchContextLocal.processWorkQueue params th globalSeen outcomesComputer queue lctx
+section
+
+-- FIXME: The proofs are also very similar to the sequential one
+
+variable {params : SearchParameters ρ σ} {th : ρ}
+  {sys : EnumerableTransitionSystem ρ (List ρ) σ (List σ) ℤ κ (List (κ × ExecutionOutcome ℤ σ)) th}
+  {lctx : MapReduceSearchContextLocal σ κ σₕ}
+  {globalSeen : Std.TreeSet σₕ}
+
+theorem MapReduceSearchContextLocalInvariants.processSuccessors_preserves_invs
+  {p : QueueItem σₕ σ → Prop}
+  {fpSt depth} (curr : σ) {succs}
+  (h_not_finished : lctx.1.finished = .none)
+  (h_reachable : sys.reachable curr)
+  (h_succs : ∀ (label : κ) (st : σ),
+    (label, st) ∈ succs ↔ (label, ExecutionOutcome.success st) ∈ sys.tr th curr)
+  (lctx_invs : MapReduceSearchContextLocalInvariants sys params globalSeen p lctx) :
+  MapReduceSearchContextLocalInvariants sys params globalSeen p (lctx.processSuccessors globalSeen fpSt depth succs) := by
+  unfold MapReduceSearchContextLocal.processSuccessors ; dsimp
+  -- need to attach some proofs
+  have htmp := List.unattach_attachWith (p := fun a => (a.1, ExecutionOutcome.success a.2) ∈ sys.tr th curr)
+    (l := succs) (H := by simp [← h_succs])
+  generalize succs.attachWith _ _ = succs' at htmp
+  rw [← htmp] ; clear htmp h_succs
+  induction succs' generalizing lctx with
+  | nil => simp ; assumption
+  | cons x succs ih =>
+    rcases x with ⟨⟨label, postState⟩, h⟩ ; dsimp [List.foldl] ; apply ih
+    · fun_cases MapReduceSearchContextLocal.tryExploreNeighbor <;> dsimp at h_not_finished <;> simp [h_not_finished]
+    · clear ih
+      fun_cases MapReduceSearchContextLocal.tryExploreNeighbor
+      on_goal 1=> cases lctx_invs ; constructor <;> assumption
+      -- enqueue case
+      rename_i ctx sq fingerprint h_not_seen ; subst fingerprint
+      simp at h_not_seen h_not_finished
+      rcases lctx_invs with ⟨⟨h_q_sound, h_vis_sound⟩, h_not_explored_all, h_dj, h_same_dom, h_succ_coll⟩ ; dsimp only at *
+      constructor ; on_goal 1=> constructor
+      all_goals dsimp only at * ; try grind
+      simp ; grind
+
+omit params th sys in
+theorem MapReduceSearchContextLocalInvariants.processSuccessors_successors_collected
+  {fpSt depth succs} :
+  letI res := lctx.processSuccessors globalSeen fpSt depth succs
+  ∀ l v, (l, v) ∈ succs.reverse → ((fp.view v) ∈ globalSeen ∨ (fp.view v) ∈ res.1.log) := by
+  unfold MapReduceSearchContextLocal.processSuccessors ; dsimp
+  -- use `foldr` to make induction easier
+  rw [List.foldl_eq_foldr_reverse]
+  generalize succs.reverse = succs
+  induction succs with
+  | nil => simp
+  | cons x succs ih =>
+    rcases x with ⟨label, postState⟩ ; dsimp [List.foldr]
+    simp only [List.mem_cons] ; introv ; intro h1 ; rcases h1 with h1 | h1
+    · injection h1 with h1 h2 ; subst l v
+      fun_cases MapReduceSearchContextLocal.tryExploreNeighbor globalSeen fpSt (depth + 1) (List.foldr _ lctx succs) label postState <;> grind
+    · rewrite (occs := .pos [1]) [MapReduceSearchContextLocal.tryExploreNeighbor]
+      split_ifs with h <;> dsimp <;> grind
+
+theorem MapReduceSearchContextLocalInvariants.processState_progress
+  {p : QueueItem σₕ σ → Prop}
+  (fpSt : σₕ) (curr : σ) (depth : Nat)
+  (h_reachable : sys.reachable curr)
+  (h_not_finished : lctx.1.finished = .none)
+  (lctx_invs : MapReduceSearchContextLocalInvariants sys params globalSeen p lctx) :
+  MapReduceSearchContextLocalInvariants sys params globalSeen (fun x => p x ∨ x = ⟨fpSt, curr, depth⟩)
+    (MapReduceSearchContextLocal.processState globalSeen params th fpSt depth curr (sys.tr th curr) lctx) := by
+  rcases lctx with ⟨ctx, q⟩ ; rcases lctx_invs with ⟨⟨h_q_sound, h_vis_sound⟩, h_not_explored_all, h_dj, h_succ_coll⟩ ; dsimp only at *
+
+  dsimp [MapReduceSearchContextLocal.processState]
+  fun_cases BaseSearchContext.processState params th fpSt curr (sys.tr th curr) ctx
+  rename_i succs exns h_eq_part hasSuccessfulTransition completedDepth newViolations
+    earlyTermination h_eq_checkvio ctx' ctx''
+  subst completedDepth ; dsimp only
+  revert h_eq_checkvio ; fun_cases checkViolationsAndMaybeTerminate params th fpSt curr ctx.completedDepth hasSuccessfulTransition exns
+  rename_i safetyViolations safetyViolation deadlock tmp1 tmp2
+  intro htmp ; injection htmp with h_eq_newvio h_eq_earlyterm ; subst tmp1 tmp2
+  -- see if early termination happened
+  rcases earlyTermination with _ | earlyTermination
+  on_goal 2=>
+    -- early termination case
+    subst ctx' ctx'' ; dsimp
+    cases earlyTermination
+    all_goals (try solve
+      | dsimp
+        constructor ; on_goal 1=> constructor
+        all_goals dsimp only at * ; try solve | assumption | grind)
+  subst ctx' ctx'' ; dsimp ; rw [h_not_finished]
+  -- normal case
+  apply MapReduceSearchContextLocalInvariants.progress_by_one_state (p := p) (curr := curr) (fpSt := fpSt) (depth := depth)
+  · apply MapReduceSearchContextLocalInvariants.processSuccessors_preserves_invs
+    · rfl
+    · exact h_reachable
+    · introv ; rw [← partitionExecutionOutcome.fst_spec, h_eq_part]
+    · constructor ; on_goal 1=> constructor
+      all_goals dsimp only at * ; try grind
+  · introv ; intro h1
+    apply MapReduceSearchContextLocalInvariants.processSuccessors_successors_collected l v
+    simp ; rw [← partitionExecutionOutcome.fst_spec, h_eq_part] at h1 ; exact h1
+  · simp
 
 end
 
-omit params th in
-def MapReduceSearchContextMain.mergeWithLocalOnes {as : List α}
-  (mctx : MapReduceSearchContextMain σ κ σₕ)
-  (lctxs : IteratedProd (as.map fun _ => MapReduceSearchContextLocal σ κ σₕ)) : MapReduceSearchContextMain σ κ σₕ :=
-  let (ctx, _, globalSeen) := mctx
-  -- CHECK There are two choices for `st`: `HashSet` or `TreeSet`. Which is better?
-  let (mbase, mq, st) := IteratedProd.foldl (elements := lctxs)
-    (init := (ctx, (#[] : Array (QueueItem σₕ σ)), (Std.HashSet.emptyWithCapacity : Std.HashSet σₕ))) fun acc r =>
-    let (mbase, mq, st) := acc
-    let (lbase, lq) := r
-    let (mq', st') := lq.foldl (init := (mq, st)) fun (mq_acc, st_acc) item =>
-      if !st_acc.contains item.fingerprint then
-        (mq_acc.push item, st_acc.insert item.fingerprint)
-      else
-        (mq_acc, st_acc)
-    ⟨mbase.mergeWithoutDepthChange lbase, mq', st'⟩
-  (mbase, mq, globalSeen.insertMany st)
-  /-
-  IteratedProd.foldl (elements := lctxs) (init := mctx) fun acc r =>
-    let ⟨mbase, mq, st⟩ := acc
-    -- TODO need to think about the semantics of `st`
-    let (lbase, lq) := r
-    let (mq', st') := lq.foldl (init := (mq, st)) fun (mq_acc, st_acc) item =>
-      if !st_acc.contains item.fingerprint then
-        (mq_acc.push item, st_acc.insert item.fingerprint)
-      else
-        (mq_acc, st_acc)
-    ⟨mbase.mergeWithoutDepthChange lbase, mq', st'⟩
-  -/
+namespace LawfulMapReduceSearchContextLocal
 
-omit th in
+-- CHECK For now, separate proofs out to reduce the risk of having weird performance
+private theorem processWorkQueue.subproof1 {α : Type u}
+  -- (p : α → Prop) : p = (fun x => p x ∨ x ∈ ([] : List α)) := by simp
+  {p q : α → Prop} (h : ∀ x, q x ↔ p x ∨ x ∈ ([] : List α)) : p = q := by simp at h ; grind
+
+private theorem processWorkQueue.subproof2 {α : Type u}
+  {p q : α → Prop} {a : α} {l : List α}
+  (h : ∀ x, q x ↔ p x ∨ x ∈ a :: l) : ∀ x, q x ↔ (p x ∨ x = a) ∨ x ∈ l := by grind
+
+omit [Ord σₕ] in
+private theorem processWorkQueue.subproof3
+  {α : Type u}
+  {a : Option α} : (¬ a.isSome = true) → a = none := by simp
+
+private theorem processWorkQueue.subproof4 {α : Type u}
+  {p : α → Prop} {a : α} {l : List α}
+  (h : ∀ x ∈ a :: l, p x) : ∀ x ∈ l, p x := by grind
+
+private theorem processWorkQueue.subproof5 {α : Type u}
+  {p : α → Prop} {a : α} {l : List α}
+  (h : ∀ x ∈ a :: l, p x) : p a := by grind
+
+private theorem processWorkQueue.subproof6 {α : Type u}
+  -- {p : α → Prop} {a : α}
+  (arr : Array α) :
+  ∀ x, x ∈ arr ↔ False ∨ x ∈ arr.toList := by grind
+
+private theorem processWorkQueue.subproof7 {α : Type u}
+  {p : α → Prop} {arr : Array α}
+  (h : ∀ x ∈ arr, p x) : ∀ x ∈ arr.toList, p x := by grind
+
+-- NOTE: A different way to reason about this is to use a subtype like
+-- `{ a // a = f b }`, where `f` is like "applying `processState` for multiple iterations".
+-- Then the proof about the invariant can be extrinsic.
+
+def processWorkQueue
+  {params : SearchParameters ρ σ} {th : ρ}
+  {sys : EnumerableTransitionSystem ρ (List ρ) σ (List σ) ℤ κ (List (κ × ExecutionOutcome ℤ σ)) th}
+  {globalSeen : Std.TreeSet σₕ}
+  (queue : List (QueueItem σₕ σ))
+  {p q : QueueItem σₕ σ → Prop} (h : ∀ x, q x ↔ p x ∨ x ∈ queue)
+  (h_inqueue_reachable : ∀ item ∈ queue, sys.reachable item.state)
+  (lctx : LawfulMapReduceSearchContextLocal (κ := κ) sys params globalSeen p) :
+    LawfulMapReduceSearchContextLocal (κ := κ) sys params globalSeen q :=
+  let ⟨v, hl⟩ := lctx
+  match queue with
+  | [] => ⟨v, (processWorkQueue.subproof1 h) ▸ hl⟩
+  | item :: rest =>
+    if h_finished : v.hasFinished
+    then ⟨v, hl.finished_change_visited_pred_in_invs h_finished⟩
+    else
+      let ⟨fpSt, curr, depth⟩ := item
+      let v' := v.processState globalSeen params th fpSt depth curr (sys.tr th curr)
+      -- CHECK Is this proper tail-recursive?
+      processWorkQueue rest
+        (processWorkQueue.subproof2 h)
+        (processWorkQueue.subproof4 h_inqueue_reachable)
+        <| Subtype.mk v' <| hl.processState_progress fpSt curr depth
+          (processWorkQueue.subproof5 (α := QueueItem σₕ σ) h_inqueue_reachable)
+          (processWorkQueue.subproof3 h_finished)
+
+-- TODO need to fix this `toList` later
+
+/-- Main worker entry point. Creates a neutral context and processes the work queue.
+    This function is called by each parallel task. -/
+def bfsBigStep
+  [Monad m] [MonadLiftT BaseIO m] [MonadLiftT IO m]
+  (params : SearchParameters ρ σ) {th : ρ}
+  (sys : EnumerableTransitionSystem ρ (List ρ) σ (List σ) ℤ κ (List (κ × ExecutionOutcome ℤ σ)) th)
+  (globalSeen : Std.TreeSet σₕ)
+  (completedDepth : Nat)
+  (queue : Array (QueueItem σₕ σ))
+  (h_inqueue_reachable : ∀ item ∈ queue, sys.reachable item.state) :
+  m (LawfulMapReduceSearchContextLocal (κ := κ) sys params globalSeen (· ∈ queue)) :=
+  let lctx : LawfulMapReduceSearchContextLocal sys params globalSeen (fun _ => False) :=
+    ⟨MapReduceSearchContextLocal.initial completedDepth, MapReduceSearchContextLocalInvariants.initial sys params globalSeen completedDepth⟩
+  let res := lctx.processWorkQueue queue.toList
+    (processWorkQueue.subproof6 queue)
+    (processWorkQueue.subproof7 h_inqueue_reachable)
+  pure res
+
+end LawfulMapReduceSearchContextLocal
+
+@[inline]
+def MapReduceSearchContextTemp.mergeOne.innerMerge
+  (acc : Array (QueueItem σₕ σ) × Std.HashSet σₕ) (item : QueueItem σₕ σ) :
+  Array (QueueItem σₕ σ) × Std.HashSet σₕ :=
+  let (mq_acc, st_acc) := acc
+  if !st_acc.contains item.fingerprint then
+    (mq_acc.push item, st_acc.insert item.fingerprint)
+  else
+    (mq_acc, st_acc)
+
+def MapReduceSearchContextTemp.mergeOne.innerMergeDescription
+  (acc res : Array (QueueItem σₕ σ) × Std.HashSet σₕ) (inQ : QueueItem σₕ σ → Prop) : Prop :=
+  ∃ suffix, res.1 = acc.1 ++ suffix ∧
+    (suffix.map QueueItem.fingerprint).toList.Nodup ∧
+    -- subsequence?
+    -- (∀ item, item ∈ suffix ↔ item ∈ lq ∧ item.fingerprint ∉ acc.2) ∧
+    (∀ fp, (∃ item, inQ item ∧ item.fingerprint = fp) → fp ∉ acc.2 →
+      fp ∈ (suffix.map QueueItem.fingerprint)) ∧
+    (∀ item ∈ suffix, inQ item ∧ item.fingerprint ∉ acc.2) ∧
+    (∀ fp, fp ∈ res.2 ↔ fp ∈ acc.2 ∨ fp ∈ (suffix.map QueueItem.fingerprint))
+
+omit [Ord σₕ] in
+theorem MapReduceSearchContextTemp.mergeOne.innerMergeDescription.concat
+  {p q : QueueItem σₕ σ → Prop} {a1 a2 a3}
+  (h1 : mergeOne.innerMergeDescription a1 a2 p) (h2 : mergeOne.innerMergeDescription a2 a3 q) :
+  mergeOne.innerMergeDescription a1 a3 fun x => p x ∨ q x := by
+  rcases h1 with ⟨suffix1, h_suffix1, h_nodup1, h_inQ1, h_fps1⟩
+  rcases h2 with ⟨suffix2, h_suffix2, h_nodup2, h_inQ2, h_fps2⟩
+  exists (suffix1 ++ suffix2) ; grind
+
+omit [Ord σₕ] in
+theorem MapReduceSearchContextTemp.mergeOne.innerMerge_foldl_descriptive
+  (acc : Array (QueueItem σₕ σ) × Std.HashSet σₕ) (lq : Array (QueueItem σₕ σ)) :
+  let res := lq.foldl (init := acc) mergeOne.innerMerge
+  mergeOne.innerMergeDescription acc res (· ∈ lq) := by
+  dsimp only [innerMergeDescription]
+  rw [← Array.foldl_toList] ; generalize hll : lq.toList = lq'
+  simp only [← Array.mem_toList_iff (xs := lq), hll] ; clear lq hll
+  induction lq' generalizing acc with
+  | nil => exists #[] ; simp [List.foldl]
+  | cons item lq' ih =>
+    dsimp [List.foldl]
+    specialize ih (mergeOne.innerMerge acc item)
+    revert ih ; fun_cases mergeOne.innerMerge acc item
+    · intro ih ; rcases ih with ⟨suffix, h_suffix, h_nodup, h_subseq, h_fps⟩
+      rename_i mq_acc st_acc hh ; simp at *
+      exists (#[item] ++ suffix) ; simp ; split_ands <;> try grind
+    · grind
+
+@[inline]
+def MapReduceSearchContextTemp.mergeOne
+  (acc : MapReduceSearchContextTemp σ κ σₕ) (lctx : MapReduceSearchContextLocal σ κ σₕ) :
+  MapReduceSearchContextTemp σ κ σₕ :=
+  let ⟨mbase, mq, st⟩ := acc
+  let (lbase, lq) := lctx
+  let (mq', st') := lq.foldl (init := (mq, st)) mergeOne.innerMerge
+  ⟨mbase.mergeWithoutDepthChange lbase, mq', st'⟩
+
+omit [Ord σₕ] in
+theorem MapReduceSearchContextTemp.mergeOne_foldl_descriptive
+  (acc : MapReduceSearchContextTemp σ κ σₕ) (lctxs : List (MapReduceSearchContextLocal σ κ σₕ)) :
+  let res := lctxs.foldl (init := acc) MapReduceSearchContextTemp.mergeOne
+  res.base = (lctxs.map Prod.fst).foldl (init := acc.base) BaseSearchContext.mergeWithoutDepthChange ∧
+  mergeOne.innerMergeDescription (acc.tovisit, acc.tempSeen) (res.tovisit, res.tempSeen)
+    (∃ lctx ∈ lctxs, · ∈ lctx.2) := by
+  dsimp only
+  induction lctxs generalizing acc with
+  | nil =>
+    constructor
+    · rfl
+    · exists #[] ; simp [List.foldl]
+  | cons lctx lctxs ih =>
+    dsimp [List.foldl]
+    specialize ih (mergeOne acc lctx) ; rcases ih with ⟨ih1, ih2⟩
+    constructor
+    · rw [ih1] ; rfl
+    · have hh := mergeOne.innerMerge_foldl_descriptive (acc.tovisit, acc.tempSeen) lctx.2
+      rewrite (occs := .pos [1, 2]) [mergeOne] at ih2
+      set e := lctx.2.foldl mergeOne.innerMerge (acc.tovisit, acc.tempSeen)
+      rcases e with ⟨mq_acc, st_acc⟩ ; dsimp at hh ih2
+      have htmp := mergeOne.innerMergeDescription.concat hh ih2
+      simp only [List.mem_cons, exists_eq_or_imp] ; exact htmp
+
+omit [Ord σₕ] in
+theorem BaseSearchContext.mergeWithoutDepthChange_foldl_description
+  (acc : BaseSearchContext σ κ σₕ) (ctxs : List (BaseSearchContext σ κ σₕ)) :
+  let res := ctxs.foldl (init := acc) BaseSearchContext.mergeWithoutDepthChange
+  res.finished = acc.finished.or ((ctxs.find? (·.hasFinished)).bind (fun x => x.finished)) := by
+  dsimp only
+  induction ctxs generalizing acc with
+  | nil => simp [List.foldl]
+  | cons ctx ctxs ih =>
+    dsimp [List.foldl, List.find?, BaseSearchContext.hasFinished]
+    rw [ih] ; clear ih
+    unfold mergeWithoutDepthChange ; dsimp
+    rcases acc.finished with _ | _
+    on_goal 2=> rfl
+    dsimp ; rcases h : ctx.finished with _ | _
+    on_goal 2=> grind
+    dsimp ; rfl
+
+def MapReduceSearchContextMain.mergeWithLocalOnes
+  {params : SearchParameters ρ σ} {th : ρ}
+  {sys : EnumerableTransitionSystem ρ (List ρ) σ (List σ) Int κ (List (κ × ExecutionOutcome Int σ)) th}
+  (mctx : MapReduceSearchContextMain σ κ σₕ)
+  {splitArrays : List (Array (QueueItem σₕ σ))}
+  {globalSeen : Std.TreeSet σₕ}
+  (lctxs : IteratedProd (splitArrays.map fun a => LawfulMapReduceSearchContextLocal (κ := κ) sys params globalSeen (· ∈ a))) :
+  MapReduceSearchContextMain σ κ σₕ :=
+  let ⟨ctx, q, globalSeen⟩ := mctx
+  -- CHECK There are two choices for `st`: `HashSet` or `TreeSet`. Which is better?
+  let ⟨mbase, mq, st⟩ := IteratedProd.foldl (β := MapReduceSearchContextTemp σ κ σₕ) (elements := lctxs)
+    (init := ⟨ctx, q, (Std.HashSet.emptyWithCapacity : Std.HashSet σₕ)⟩)
+      fun acc lctx => acc.mergeOne lctx.val
+  ⟨mbase, mq, globalSeen.insertMany st⟩
+
+private theorem List.zip_mem {α : Type u} {β : Type v} {l1 : List α} {l2 : List β}
+  (hl : l1.length ≤ l2.length) (h : i < l1.length) :
+  (l1[i], l2[i]) ∈ l1.zip l2 := by
+  induction l1 generalizing i l2 with
+  | nil => simp at h
+  | cons a l1 ih =>
+    cases l2 with
+    | nil => simp at hl
+    | cons b l2 =>
+      cases i with
+      | zero => exact .head _
+      | succ i =>
+        simp only [List.length_cons] at hl h
+        exact .tail _ (ih (by omega) (by omega))
+
+theorem MapReduceSearchContextMain.mergeWithLocalOnes_preserves_invs
+  [Std.TransOrd σₕ] [Std.LawfulBEqOrd σₕ]
+  {params : SearchParameters ρ σ} {th : ρ}
+  {sys : EnumerableTransitionSystem ρ (List ρ) σ (List σ) Int κ (List (κ × ExecutionOutcome Int σ)) th}
+  {mctx : MapReduceSearchContextMain σ κ σₕ}
+  (h_not_finished : mctx.base.hasFinished = false)
+  (h_mctx : MapReduceSearchContextMainInvariants sys params mctx)
+  (lctxs :
+    let ranges := ParallelConfig.chunkRanges parallelCfg mctx.tovisit.size
+    let splitArrays := ranges.map fun lr => mctx.tovisit.extract lr.1 lr.2
+    IteratedProd (splitArrays.map fun a => LawfulMapReduceSearchContextLocal (κ := κ) sys params mctx.globalSeen (· ∈ a))) :
+  let mctx' := MapReduceSearchContextMain.mergeWithLocalOnes ⟨mctx.base, #[], mctx.globalSeen⟩ lctxs
+  MapReduceSearchContextMainInvariants sys params mctx' := by
+  rcases mctx with ⟨ctx, tovisit, gs⟩
+  dsimp ; unfold mergeWithLocalOnes
+  simp only [IteratedProd.subtypesToList_foldl_eq_list_foldl]
+  have h_local_invs := IteratedProd.externalize_proofs lctxs ; dsimp at h_local_invs
+  rcases h_local_invs with ⟨h_length_eq, h_local_invs⟩
+  generalize IteratedProd.subtypesToList lctxs = lctxs' at *
+  set merged := lctxs'.foldl _ _ with heq
+  have htmp2 := ({ base := ctx, tovisit := #[], tempSeen := Std.HashSet.emptyWithCapacity : MapReduceSearchContextTemp σ κ σₕ }).mergeOne_foldl_descriptive lctxs'
+  dsimp at htmp2 ; rw [← heq] at htmp2 ; rcases htmp2 with ⟨h_base, h_merge_desc⟩
+  have h_base_desc := BaseSearchContext.mergeWithoutDepthChange_foldl_description ctx (lctxs'.map Prod.fst)
+  simp [BaseSearchContext.hasFinished] at h_not_finished
+  dsimp at h_base_desc ; rw [← h_base, h_not_finished] at h_base_desc ; dsimp at h_base_desc
+  clear lctxs heq h_base ; clear_value merged
+
+  rcases merged with ⟨mbase, mq, st⟩
+  rcases h_merge_desc with ⟨suffix, h_suffix, h_nodup, h_in_suffix, h_inQ, h_fps⟩
+  dsimp only at * ; subst mq
+  simp at h_inQ h_fps h_in_suffix ; simp at h_local_invs
+
+  rcases h_mctx with ⟨⟨h_q_sound, h_vis_sound⟩, h_init_incl, h_q_emp, h_closed⟩
+  whnf at h_closed ; dsimp only at *
+  clear h_q_emp
+
+  -- prove a lemma first, since it will be used in both `terminate_empty_queue` and `stable_closed`
+  have h_not_explored_all : mbase.finished ≠ Option.some (TerminationReason.exploredAllReachableStates) := by
+    intro h ; rw [h_base_desc, Option.bind_eq_some_iff] at h ; simp +unfoldPartialApp [Function.comp] at h
+    rcases h with ⟨lbctx, ⟨⟨lq, h_find⟩, h_finished⟩⟩
+    -- deriving false here
+    rw [List.find?_eq_some_iff_getElem] at h_find
+    rcases h_find with ⟨_, i, h_i, h_getElem, _⟩
+    -- NOTE: This is repeating
+    have h_in_zip := List.zip_mem (by apply Nat.le_of_eq ; symm ; apply h_length_eq) (by rw [← h_length_eq] ; apply h_i)
+    rw [h_getElem] at h_in_zip
+    specialize h_local_invs _ _ _ h_in_zip
+    have := h_local_invs.not_explored_all ; grind
+
+  constructor ; on_goal 1=> constructor
+  · simp
+    intro fpSt curr depth hh
+    specialize h_inQ _ hh
+    rcases h_inQ with ⟨lbctx, lq, h_in_lctxs', h_in_q⟩
+    -- This is annoying ...
+    rw [List.mem_iff_getElem] at h_in_lctxs'
+    rcases h_in_lctxs' with ⟨i, h_i, h_getElem⟩
+    have h_in_zip := List.zip_mem (by apply Nat.le_of_eq ; symm ; apply h_length_eq) (by rw [← h_length_eq] ; apply h_i)
+    rw [h_getElem] at h_in_zip
+    specialize h_local_invs _ _ _ h_in_zip
+    rcases h_local_invs with ⟨⟨h_q_sound, h_vis_sound⟩, h_not_explored_all, h_dj, h_same_dom, h_succ_coll⟩ ; dsimp only at *
+    grind
+  · simp
+    intro hinj x hh ; rcases hh with hh | hh
+    · grind
+    · rw [h_fps] at hh ; rcases hh with ⟨⟨fpSt, curr, depth⟩, hh, heq⟩ ; dsimp at heq ; subst fpSt
+      -- NOTE: This is repeating
+      specialize h_inQ _ hh
+      rcases h_inQ with ⟨lbctx, lq, h_in_lctxs', h_in_q⟩
+      rw [List.mem_iff_getElem] at h_in_lctxs'
+      rcases h_in_lctxs' with ⟨i, h_i, h_getElem⟩
+      have h_in_zip := List.zip_mem (by apply Nat.le_of_eq ; symm ; apply h_length_eq) (by rw [← h_length_eq] ; apply h_i)
+      rw [h_getElem] at h_in_zip
+      specialize h_local_invs _ _ _ h_in_zip
+      rcases h_local_invs with ⟨⟨h_q_sound, h_vis_sound⟩, h_not_explored_all, h_dj, h_same_dom, h_succ_coll⟩ ; dsimp only at *
+      grind
+  · simp ; grind
+  · simp ; grind
+  · whnf ; simp
+    intro hinj hor u hh h_not_in_suffix
+    rcases hor with _ | h_not_finished_mbase
+    on_goal 1=> grind
+    rcases hh with hh | hh
+    · by_cases h_in_tovisit? : (∀ item ∈ tovisit, item.fingerprint ≠ StateView.view u)
+      · grind  -- easy case
+      · clear h_closed
+        simp at h_in_tovisit? ; rcases h_in_tovisit? with ⟨⟨fpSt, curr, depth⟩, h_in_tovisit, heq⟩
+        dsimp at heq ; subst fpSt
+        have := hinj (h_q_sound _ _ _ h_in_tovisit |>.right.right) ; subst curr -- unify `curr` with `u`
+        rw [Array.mem_iff_getElem] at h_in_tovisit
+        rcases h_in_tovisit with ⟨i, h_i, h_getElem_tovisit⟩
+        -- here, need the split covering theorem
+        obtain ⟨⟨li, ri⟩, h_chunk_in, h_in_interval⟩ := ParallelConfig.chunkRanges_cover parallelCfg tovisit.size _ h_i
+        dsimp at h_in_interval ; rcases h_in_interval with ⟨h_li, h_ri⟩
+        rw [List.mem_iff_getElem] at h_chunk_in
+        rcases h_chunk_in with ⟨j, h_j, h_getElem_chunk⟩
+        have h_in_zip := List.zip_mem (by apply Nat.le_of_eq ; symm ; apply h_length_eq) (by simp ; apply h_j)
+        simp [h_getElem_chunk] at h_in_zip
+        specialize h_local_invs _ _ _ h_in_zip ; simp at h_local_invs
+        -- show that no `lctx` has finished
+        rw [h_base_desc] at h_not_finished_mbase
+        revert h_not_finished_mbase ; rcases heq : List.find? _ _ with _ | lctx
+        on_goal 2=>
+          dsimp ; intro heq' ; rw [List.find?_eq_some_iff_getElem, BaseSearchContext.hasFinished] at heq ; grind
+        intro _ ; simp at heq
+        -- NOTE: Here Lean has some trouble proving the index validity of `j` from the scratch, so use some trick
+        set e := getElem lctxs' j _
+        specialize heq e.1 e.2 (by simp [e]) ; simp [BaseSearchContext.hasFinished] at heq
+        rcases h_local_invs with ⟨_, _, h_dj, h_same_dom, h_succ_coll⟩
+        specialize h_succ_coll heq (StateView.view u) u depth (by
+          rw [← h_getElem_tovisit, Array.mem_extract_iff_getElem]
+          exists (i - li) ; simp [h_li] ; omega)
+        grind
+    · grind
+
+omit [BEq κ] [Hashable κ] in
+private theorem breadthFirstSearchParallel.subproof1 {ρ σₕ σ : Type}
+  [fp : StateFingerprint σ σₕ]
+  {th : ρ}
+  {sys : EnumerableTransitionSystem ρ (List ρ) σ (List σ) Int κ (List (κ × ExecutionOutcome Int σ)) th}
+  {seen : σₕ → Prop}
+  {tovisit : Array (QueueItem σₕ σ)}
+  (h : ∀ x st d, ⟨x, st, d⟩ ∈ tovisit → sys.reachable st ∧ seen x ∧ x = fp.view st)
+  (ranges : List (Nat × Nat)) :
+  ∀ subarr ∈ (ranges.map fun lr => tovisit.extract lr.1 lr.2),
+    ∀ item ∈ subarr, sys.reachable item.state := by
+  intro subarr h_subarr_in item h_item_in
+  specialize h item.fingerprint item.state item.depth ; rw [← QueueItem.fold_unfold] at h
+  obtain ⟨lr, _, h_subarr_eq⟩ := List.mem_map.mp h_subarr_in
+  rw [← h_subarr_eq, Array.mem_extract_iff_getElem] at h_item_in
+  grind
+
 def breadthFirstSearchParallel {m : Type → Type}
   [Monad m] [MonadLiftT BaseIO m] [MonadLiftT IO m]
   [Repr κ]
+  [Std.TransOrd σₕ] [Std.LawfulBEqOrd σₕ]
+  (params : SearchParameters ρ σ)
   {th : ρ}
   (sys : EnumerableTransitionSystem ρ (List ρ) σ (List σ) Int κ (List (κ × ExecutionOutcome Int σ)) th)
   (parallelCfg : ParallelConfig)
   (progressInstanceId : Nat)
   (cancelToken : IO.CancelToken) :
   m (MapReduceSearchContextMain σ κ σₕ) := do
-  let mut mctx : MapReduceSearchContextMain σ κ σₕ := MapReduceSearchContextMain.initial sys
+  let mut mctx : LawfulMapReduceSearchContextMain (fp := fp) sys params :=
+    Subtype.mk (MapReduceSearchContextMain.initial sys.initStates) (MapReduceSearchContextMainInvariants.initial sys params)
   let mut lastUpdateTime : Nat := 0
   let mut cancelled := false
-  while h_not_finished : mctx.hasFinished = false do
-    -- FIXME: Need to add a sequential fallback if the frontier is too small
+  while h_not_finished : mctx.val.base.hasFinished = false do
     match mctx with
-    | (base, tovisitArr, globalSeen) =>
+    | ⟨⟨base, tovisit, globalSeen⟩, h_mctx⟩ =>
       -- Check if the frontier is empty
-      if tovisitArr.isEmpty then
-        mctx := ({ base with finished := some (.exploredAllReachableStates) }, tovisitArr, globalSeen)
+      if h_empty : tovisit.isEmpty then
+        mctx := Subtype.mk ⟨{ base with finished := some (.exploredAllReachableStates) }, tovisit, globalSeen⟩
+          (h_mctx.setExploredAll_preserves_invs h_not_finished h_empty)
         break
       else
+        -- FIXME: Need to add a proper sequential fallback if the frontier is too small
         -- Compute chunk ranges for splitting the work
-        let ranges := ParallelConfig.chunkRanges parallelCfg tovisitArr.size
+        let ranges := ParallelConfig.chunkRanges parallelCfg tovisit.size
         -- Split the queue into sub-arrays of `QueueItems`
-        -- Use `Subarray` to avoid copying the data for each chunk
-        let splitArrays := ranges.map fun lr => tovisitArr.extract lr.1 lr.2
+        let splitArrays := ranges.map fun lr => tovisit.extract lr.1 lr.2
         let completedDepth := base.completedDepth
         -- Map step: spawn parallel tasks
         -- **CAVEAT**: The call to `IO.asTask` **SHOULD NOT** be put in this procedure,
         -- as that might cause parallelism to vanish!!! Instead, the call should be defined
         -- in some other file.
-        let tasks ← IteratedProd.taskSplit splitArrays fun subArr _ =>
-          (pure (MapReduceSearchContextLocal.bfsBigStep params th globalSeen sys.tr completedDepth subArr) : IO _)
-        let results ← IteratedProd.mapM (fun task => IO.ofExcept task.get) tasks
+        let tasks ← IteratedProd.taskSplit splitArrays fun subArr h_subarr_in =>
+          LawfulMapReduceSearchContextLocal.bfsBigStep params sys globalSeen completedDepth subArr
+            (breadthFirstSearchParallel.subproof1 h_mctx.queue_sound ranges _ h_subarr_in)
+        let results ← IteratedProd.mapM
+          (T₂ := (fun a => LawfulMapReduceSearchContextLocal sys params globalSeen (· ∈ a)))
+          (fun task => IO.ofExcept task.get) tasks
+        -- CHECK Ideally, `tovisit` should not be involved in any computational part from this point on
         -- Reduce step
-        -- CHECK rewrite into a bind to prevent the reuse of `base` and `tovisitArr`?
-        let mctx' := mctx.mergeWithLocalOnes results
-
-        match mctx' with
-        | (base', tovisitArr', globalSeen') =>
+        let mctxValForMerge : MapReduceSearchContextMain σ κ σₕ := ⟨base, #[], globalSeen⟩
+        let mctxVal' := mctxValForMerge.mergeWithLocalOnes results
+        have h_mctx' : MapReduceSearchContextMainInvariants sys params mctxVal' :=
+          MapReduceSearchContextMain.mergeWithLocalOnes_preserves_invs h_not_finished h_mctx results
+        match heq : mctxVal' with
+        | ⟨base', tovisit', globalSeen'⟩ =>
           trySetViolationFound progressInstanceId base'
           -- Update progress on every diameter change
-          updateProgressDuringBFS progressInstanceId base' tovisitArr'.size
-          mctx := (base', tovisitArr', globalSeen')
+          updateProgressDuringBFS progressInstanceId base' tovisit'.size
+          -- Prove invariants are preserved using local invariants from `lawfulResults`
+          mctx := Subtype.mk ⟨base', tovisit', globalSeen'⟩ (heq.symm ▸ h_mctx')
           -- Check for cancellation/handoff at most once per second
           let newtime? ← checkCancellationWithoutPeriodicUpdate progressInstanceId lastUpdateTime 1000 cancelToken
           match newtime? with
@@ -171,11 +573,11 @@ def breadthFirstSearchParallel {m : Type → Type}
           | .searchCancelled => cancelled := true ; break
           | .noUpdate => pure ()
   -- Final update to ensure stats reflect finished state
-  updateProgressDuringBFS progressInstanceId mctx.1 mctx.2.1.size
+  let ⟨mctxVal, _⟩ := mctx
+  updateProgressDuringBFS progressInstanceId mctxVal.base mctxVal.tovisit.size
   if cancelled then
-    let mctx' := ({ mctx.1 with finished := some (.earlyTermination .cancelled) }, mctx.2)
-    return mctx'
+    return { mctxVal with base := { mctxVal.base with finished := some (.earlyTermination .cancelled) } }
   else
-    return mctx
+    return mctxVal
 
 end Veil.ModelChecker.Concrete
