Veil/Core/Tools/ModelChecker/ConcreteNew/SearchContext.lean
@@ -45,58 +45,75 @@ where
 abbrev LawfulSequentialSearchContext (stateInTransit : Option σ := .none) : Type :=
   Subtype (α := SequentialSearchContext σ κ σₕ) (SequentialSearchContextInvariants sys params stateInTransit)
 
-/-- When finishing processing a state, we move from having that state `curr`
-in transit to having no state in transit, provided that all successfully
-reachable neighbors of `curr` in transit have been seen. -/
-theorem SequentialSearchContextInvariants.finish_stateInTransit
-  {sctx : SequentialSearchContext σ κ σₕ}
-  {curr : σ}
-  (sctx_invs : SequentialSearchContextInvariants sys params (.some curr) sctx)
-  (h_neighbors_seen : ∀ l v, (l, ExecutionOutcome.success v) ∈ sys.tr th curr →
-    (fp.view v) ∈ sctx.1.log) :
-  SequentialSearchContextInvariants sys params .none sctx := by
-  rcases sctx with ⟨ctx, sq⟩ ; rcases sctx_invs with ⟨h1, h2, h3, h_closed⟩ ; dsimp only at *
-  constructor <;> try assumption
-  simp [SequentialSearchContext.isStableClosed] at h_closed ⊢
-  intro ha hb u hc hd l v hin
-  by_cases heq : curr = u
-  on_goal 2=> grind
-  subst u ; eapply h_neighbors_seen ; assumption
-
 end Sequential
 
 section MapReduce
 
 -- FIXME: The depth information in `QueueItem` is more or less useless here
 
-/-
-structure MapReduceSearchContextMain (σ κ σₕ : Type) [fp : StateFingerprint σ σₕ] [BEq κ] [Hashable κ] where
+structure MapReduceSearchContextMain (σ κ σₕ : Type) [fp : StateFingerprint σ σₕ] [Ord σₕ] [BEq κ] [Hashable κ] where
   base : BaseSearchContext σ κ σₕ
-  -- CHECK I strongly suspect there is some bad memory usage here ...
-  /-- Recording the nodes to visit in the next depth as an Array for efficient iteration/splitting. -/
-  tovisitQueue : Array (QueueItem σₕ σ)
-  /-- HashSet for O(1) membership checking of fingerprints in the queue. -/
-  tovisitSet : Std.HashSet σₕ
--/
-
-abbrev MapReduceSearchContextMain (σ κ σₕ : Type) [fp : StateFingerprint σ σₕ] [Ord σₕ] [BEq κ] [Hashable κ] :=
-  BaseSearchContext σ κ σₕ × Array (QueueItem σₕ σ) × Std.TreeSet σₕ
+  tovisit : Array (QueueItem σₕ σ)
+  globalSeen : Std.TreeSet σₕ
 
 abbrev MapReduceSearchContextLocal (σ κ σₕ : Type) [fp : StateFingerprint σ σₕ] [BEq κ] [Hashable κ] :=
   BaseSearchContext σ κ σₕ × Array (QueueItem σₕ σ)
 
+structure MapReduceSearchContextTemp (σ κ σₕ : Type) [fp : StateFingerprint σ σₕ] [BEq κ] [Hashable κ] where
+  base : BaseSearchContext σ κ σₕ
+  tovisit : Array (QueueItem σₕ σ)
+  tempSeen : Std.HashSet σₕ
+
 variable {ρ σ κ σₕ : Type}
   [fp : StateFingerprint σ σₕ]
   [instBEq : BEq κ] [instHash : Hashable κ]
+  [Ord σₕ]
   {th : ρ}
   (sys : EnumerableTransitionSystem ρ (List ρ) σ (List σ) Int κ (List (κ × ExecutionOutcome Int σ)) th)
   (params : SearchParameters ρ σ)
 
--- structure MapReduceSearchContextMainInvariants
---   (mmctx : MapReduceSearchContextMain σ κ σₕ)
--- extends @SearchContextInvariants ρ σ κ σₕ fp th sys params (· ∈ mmctx.tovisitQueue) (· ∈ mmctx.base.log)
--- where
-  -- tovisitConsistent : ∀ h, h ∈ tovisitSet ↔ ∃ item ∈ tovisitQueue, item.fingerprint = h
+/-- A map-reduce main context is stable closed if for any state `u` that
+has been seen (in globalSeen) and has been fully processed (i.e., not in the
+frontier array), then all its successfully reachable states have also been seen. -/
+abbrev MapReduceSearchContextMain.isStableClosed (mctx : MapReduceSearchContextMain σ κ σₕ) : Prop :=
+  Function.Injective fp.view →
+    (mctx.base.finished = some (.exploredAllReachableStates) ∨ mctx.base.finished = none) →
+      ∀ u, (fp.view u) ∈ mctx.globalSeen →
+        (∀ item ∈ mctx.tovisit, item.fingerprint ≠ fp.view u) →
+          ∀ l v, (l, ExecutionOutcome.success v) ∈ sys.tr th u →
+            (fp.view v) ∈ mctx.globalSeen
+
+structure MapReduceSearchContextMainInvariants
+  (mctx : MapReduceSearchContextMain σ κ σₕ)
+extends @SearchContextInvariants ρ σ κ σₕ fp th sys params (· ∈ mctx.tovisit) (· ∈ mctx.globalSeen)
+where
+  init_states_included : ∀ s ∈ sys.initStates, (fp.view s) ∈ mctx.globalSeen
+  terminate_empty_queue : mctx.base.finished = some (.exploredAllReachableStates) → mctx.tovisit.isEmpty
+  stable_closed : mctx.isStableClosed sys
+
+abbrev LawfulMapReduceSearchContextMain : Type :=
+  Subtype (α := MapReduceSearchContextMain σ κ σₕ) (MapReduceSearchContextMainInvariants sys params)
+
+structure MapReduceSearchContextLocalInvariants
+  (globalSeen : Std.TreeSet σₕ)
+  (visited : QueueItem σₕ σ → Prop)
+  (lctx : MapReduceSearchContextLocal σ κ σₕ)
+extends @SearchContextInvariants ρ σ κ σₕ fp th sys params (· ∈ lctx.2) (fun h => ∃ s d, ⟨h, s, d⟩ ∈ lctx.2)
+where
+  not_explored_all : lctx.1.finished ≠ some (.exploredAllReachableStates)   -- OK, but why?
+  tovisit_globalSeen_disjoint : ∀ item ∈ lctx.2, item.fingerprint ∉ globalSeen
+  -- NOTE: This might be eventually removed
+  tovisit_log_same_domain : ∀ fpSt, fpSt ∈ lctx.1.log ↔ ∃ item ∈ lctx.2, item.fingerprint = fpSt
+  successor_collected : lctx.1.finished = none → ∀ fingerprint st d, visited ⟨fingerprint, st, d⟩ →
+    ∀ (l : κ) (v : σ), (l, .success v) ∈ sys.tr th st →
+      ((fp.view v) ∈ globalSeen ∨
+        -- ∃ d, ⟨fp.view v, v, d⟩ ∈ lctx.1.log)
+        fp.view v ∈ lctx.1.log)
+
+abbrev LawfulMapReduceSearchContextLocal
+  (globalSeen : Std.TreeSet σₕ)
+  (visited : QueueItem σₕ σ → Prop) : Type :=
+  Subtype (α := MapReduceSearchContextLocal σ κ σₕ) (MapReduceSearchContextLocalInvariants sys params globalSeen visited)
 
 end MapReduce
 
