Veil/Core/Tools/ModelChecker/ConcreteNew/SequentialLemmas.lean
@@ -17,6 +17,24 @@ theorem SequentialSearchContextInvariants.initial :
   constructor ; on_goal 1=> constructor
   all_goals simp [SequentialSearchContext.isStableClosed, SequentialSearchContext.initial, BaseSearchContext.initial, ← fQueue.mem_ofList] ; (try solve | intros ; grind)
 
+/-- When finishing processing a state, we move from having that state `curr`
+in transit to having no state in transit, provided that all successfully
+reachable neighbors of `curr` in transit have been seen. -/
+theorem SequentialSearchContextInvariants.finish_stateInTransit
+  {sctx : SequentialSearchContext σ κ σₕ}
+  {curr : σ}
+  (sctx_invs : SequentialSearchContextInvariants sys params (.some curr) sctx)
+  (h_neighbors_seen : ∀ l v, (l, ExecutionOutcome.success v) ∈ sys.tr th curr →
+    (fp.view v) ∈ sctx.1.log) :
+  SequentialSearchContextInvariants sys params .none sctx := by
+  rcases sctx with ⟨ctx, sq⟩ ; rcases sctx_invs with ⟨h1, h2, h3, h_closed⟩ ; dsimp only at *
+  constructor <;> try assumption
+  simp [SequentialSearchContext.isStableClosed] at h_closed ⊢
+  intro ha hb u hc hd l v hin
+  by_cases heq : curr = u
+  on_goal 2=> grind
+  subst u ; eapply h_neighbors_seen ; assumption
+
 theorem SequentialSearchContext.bfs_completeness
   {sctx : SequentialSearchContext σ κ σₕ}
   (sctx_invs : SequentialSearchContextInvariants sys params .none sctx)
